git/abentkamp/duper/Duper/Saturate.lean
@@ -9,6 +9,7 @@ import Duper.Rules.ClausifyPropEq
 import Duper.Rules.EqualityResolution
 import Duper.Rules.SyntacticTautologyDeletion1
 import Duper.Rules.SyntacticTautologyDeletion2
+import Duper.Rules.SyntacticTautologyDeletion3
 import Duper.Rules.ElimDupLit
 import Duper.Rules.Demodulation
 import Duper.Rules.ElimResolvedLit
@@ -31,6 +32,7 @@ open RuleM
 initialize
   registerTraceClass `Simp
   registerTraceClass `Simp.debug
+  registerTraceClass `Timeout.debug
 
 set_option trace.Prover.debug true
 
@@ -38,39 +40,44 @@ set_option maxHeartbeats 10000
 
 open SimpResult
 
-def simpRules : ProverM (Array SimpRule) := do
+def forwardSimpRules : ProverM (Array SimpRule) := do
   return #[
-    (forwardDemodulation (← getDemodSidePremiseIdx)).toSimpRule "forward demodulation (rewriting of positive/negative literals)",
+    --(forwardDemodulation (← getDemodSidePremiseIdx)).toSimpRule "forward demodulation (rewriting of positive/negative literals)",
     clausificationStep.toSimpRule "clausification",
     syntacticTautologyDeletion1.toSimpRule "syntactic tautology deletion 1",
     syntacticTautologyDeletion2.toSimpRule "syntactic tautology deletion 2",
+    syntacticTautologyDeletion3.toSimpRule "syntactic tautology deletion 3",
     elimDupLit.toSimpRule "eliminate duplicate literals",
     elimResolvedLit.toSimpRule "eliminate resolved literals",
     destructiveEqualityResolution.toSimpRule "destructive equality resolution",
     identBoolFalseElim.toSimpRule "identity boolean false elimination"
   ]
 
-def applySimpRules (givenClause : Clause) :
-    ProverM (SimpResult Clause) := do
-  for simpRule in ← simpRules do
+def applyForwardSimpRules (givenClause : Clause) : ProverM (SimpResult Clause) := do
+  for simpRule in ← forwardSimpRules do
     match ← simpRule givenClause with
     | Removed => return Removed
     | Applied c => return Applied c
     | Unapplicable => continue
   return Unapplicable
 
-partial def simpLoop (givenClause : Clause) : ProverM (Option Clause) := do
-  Core.checkMaxHeartbeats "simpLoop"
-  match ← applySimpRules givenClause with
-  | Applied c => 
-    simpLoop c
+partial def forwardSimpLoop (givenClause : Clause) : ProverM (Option Clause) := do
+  Core.checkMaxHeartbeats "forwardSimpLoop"
+  match ← applyForwardSimpRules givenClause with
+  | Applied c => forwardSimpLoop c
   | Unapplicable => return some givenClause 
   | Removed => return none
 
+/-- Uses other clauses in the active set to attempt to simplify the given clause. Returns some simplifiedGivenClause if
+    forwardSimpLoop is able to use simplification rules to transform givenClause to simplifiedGivenClause. Returns none if
+    forwardSimpLoop is able to use simplification rules to show that givenClause is unneeded. -/
 def forwardSimplify (givenClause : Clause) : ProverM (Option Clause) := do
-  let c := simpLoop givenClause
+  let c := forwardSimpLoop givenClause
   c
 
+/-- Uses the givenClause to attempt to simplify other clauses in the active set. For each clause that backwardSimpLoop is
+    able to produce a simplification for, backwardSimplify removes the clause from the active set (and all discrimination trees)
+    and adds the newly simplified clause to the passive set. -/
 def backwardSimplify (givenClause : Clause) : ProverM Unit := do
   -- TODO: Add backward demodulation
   return ()
@@ -90,21 +97,22 @@ partial def saturate : ProverM Unit := do
           setResult saturated
           return LoopCtrl.abort
       trace[Prover.saturate] "### Given clause: {givenClause}"
-      let some givenClause ← forwardSimplify givenClause
-        | do
-          removeFromDiscriminationTrees givenClause
-          return LoopCtrl.next
-      trace[Prover.saturate] "### Given clause after simp: {givenClause}"
-      backwardSimplify givenClause
-      addToActive givenClause
-      performInferences givenClause
+      let some simplifiedGivenClause ← forwardSimplify givenClause
+        | return LoopCtrl.next
+      trace[Prover.saturate] "### Given clause after simp: {simplifiedGivenClause}"
+      backwardSimplify simplifiedGivenClause
+      addToActive simplifiedGivenClause
+      performInferences simplifiedGivenClause
       trace[Prover.saturate] "### New active Set: {(← getActiveSet).toArray}"
       return LoopCtrl.next
     catch
     | Exception.internal emptyClauseExceptionId _  =>
       setResult contradiction
       return LoopCtrl.abort
-    | e => throw e
+    | e =>
+      trace[Timeout.debug] "Active set at timeout: {(← getActiveSet).toArray}"
+      --trace[Timeout.debug] "All clauses at timeout: {Array.map (fun x => x.1) (← getAllClauses).toArray}"
+      throw e
 
 end ProverM
 
